notation and cleanup

thys/POPLmark/SystemFSub.thy
@@ -1,4 +1,4 @@
-(* System F with Subtyping  *)
+(* System F with SubTypeing  *)
 theory SystemFSub
   imports "Binders.MRBNF_Recursor"
     "Binders.Generic_Barendregt_Enhanced_Rule_Induction"
@@ -13,74 +13,74 @@ declare supp_id_bound[simp]
 (*type_synonym label = nat*)
 
 declare [[mrbnf_internals]]
-binder_datatype 'a "typ" =
+binder_datatype 'a "Type" =
     TyVar 'a
   | Top
-  | Fun "'a typ" "'a typ"
-  | Forall X::'a "'a typ" T::"'a typ" binds X in T
+  | Fun "'a Type" "'a Type"
+  | Forall X::'a "'a Type" T::"'a Type" binds X in T
 
 
-declare supp_swap_bound[OF cinfinite_imp_infinite[OF typ.UNIV_cinfinite], simp]
-declare typ.rrename_ids[simp] typ.rrename_id0s[simp]
+declare supp_swap_bound[OF cinfinite_imp_infinite[OF Type.UNIV_cinfinite], simp]
+declare Type.rrename_ids[simp] Type.rrename_id0s[simp]
 
-lemma rrename_typ_simps[simp]:
-  fixes f::"'a::var_typ_pre \<Rightarrow> 'a"
+lemma rrename_Type_simps[simp]:
+  fixes f::"'a::var_Type_pre \<Rightarrow> 'a"
   assumes "bij f" "|supp f| <o |UNIV::'a set|"
   shows
-    "rrename_typ f (TyVar X) = TyVar (f X)"
-    "rrename_typ f Top = Top"
-    "rrename_typ f (Fun t1 t2) = Fun (rrename_typ f t1) (rrename_typ f t2)"
-    "rrename_typ f (Forall Y T1 T2) = Forall (f Y) (rrename_typ f T1) (rrename_typ f T2)"
+    "rrename_Type f (TyVar X) = TyVar (f X)"
+    "rrename_Type f Top = Top"
+    "rrename_Type f (Fun t1 t2) = Fun (rrename_Type f t1) (rrename_Type f t2)"
+    "rrename_Type f (Forall Y T1 T2) = Forall (f Y) (rrename_Type f T1) (rrename_Type f T2)"
      apply (unfold TyVar_def Top_def Fun_def Forall_def)
      apply (rule trans)
-      apply (rule typ.rrename_cctors)
+      apply (rule Type.rrename_cctors)
        apply (rule assms)+
      defer
      apply (rule trans)
-      apply (rule typ.rrename_cctors)
+      apply (rule Type.rrename_cctors)
        apply (rule assms)+
      defer
      apply (rule trans)
-      apply (rule typ.rrename_cctors)
+      apply (rule Type.rrename_cctors)
        apply (rule assms)+
      defer
      apply (rule trans)
-      apply (rule typ.rrename_cctors)
+      apply (rule Type.rrename_cctors)
        apply (rule assms)+
      defer
-     apply (unfold map_typ_pre_def comp_def Abs_typ_pre_inverse[OF UNIV_I] map_sum.simps
+     apply (unfold map_Type_pre_def comp_def Abs_Type_pre_inverse[OF UNIV_I] map_sum.simps
         map_prod_simp id_def
       )
      apply (rule refl)+
   done
 
-lemma typ_inject:
+lemma Type_inject:
   "TyVar X = TyVar Y \<longleftrightarrow> X = Y"
   "Fun T1 T2 = Fun R1 R2 \<longleftrightarrow> T1 = R1 \<and> T2 = R2"
   "Forall X T1 T2 = Forall Y R1 R2 \<longleftrightarrow> 
-   T1 = R1 \<and> (\<exists>f. bij (f::'a::var_typ_pre \<Rightarrow> 'a) \<and> 
-   |supp f| <o |UNIV::'a set| \<and> id_on (FFVars_typ T2 - {X}) f \<and> f X = Y \<and> rrename_typ f T2 = R2)"
-    apply (unfold TyVar_def Fun_def Forall_def typ.TT_injects0
-      set3_typ_pre_def comp_def Abs_typ_pre_inverse[OF UNIV_I] map_sum.simps sum_set_simps
-      cSup_singleton Un_empty_left Un_empty_right Union_empty image_empty empty_Diff map_typ_pre_def
-      prod.map_id set2_typ_pre_def prod_set_simps prod.set_map UN_single Abs_typ_pre_inject[OF UNIV_I UNIV_I]
+   T1 = R1 \<and> (\<exists>f. bij (f::'a::var_Type_pre \<Rightarrow> 'a) \<and> 
+   |supp f| <o |UNIV::'a set| \<and> id_on (FFVars_Type T2 - {X}) f \<and> f X = Y \<and> rrename_Type f T2 = R2)"
+    apply (unfold TyVar_def Fun_def Forall_def Type.TT_injects0
+      set3_Type_pre_def comp_def Abs_Type_pre_inverse[OF UNIV_I] map_sum.simps sum_set_simps
+      cSup_singleton Un_empty_left Un_empty_right Union_empty image_empty empty_Diff map_Type_pre_def
+      prod.map_id set2_Type_pre_def prod_set_simps prod.set_map UN_single Abs_Type_pre_inject[OF UNIV_I UNIV_I]
       sum.inject prod.inject map_prod_simp
     )
   by auto
-declare typ_inject(1,2)[simp]
+declare Type_inject(1,2)[simp]
 
 corollary Forall_inject_same[simp]: "Forall X T1 T2 = Forall X S1 S2 \<longleftrightarrow> T1 = S1 \<and> T2 = S2"
-  using typ_inject(3) typ.rrename_cong_ids
+  using Type_inject(3) Type.rrename_cong_ids
   by (metis (no_types, lifting) Diff_empty Diff_insert0 id_on_insert insert_Diff)
 
 lemma Forall_rrename:
   assumes "bij \<sigma>" "|supp \<sigma>| <o |UNIV::'a set|" shows "
- (\<And>Y. Y\<in>FFVars_typ T2 - {X::'a::var_typ_pre} \<Longrightarrow> \<sigma> Y = Y) \<Longrightarrow> Forall X T1 T2 = Forall (\<sigma> X) T1 (rrename_typ \<sigma> T2)"
+ (\<And>Y. Y\<in>FFVars_Type T2 - {X::'a::var_Type_pre} \<Longrightarrow> \<sigma> Y = Y) \<Longrightarrow> Forall X T1 T2 = Forall (\<sigma> X) T1 (rrename_Type \<sigma> T2)"
   apply (unfold Forall_def)
-  apply (unfold typ.TT_injects0)
-  apply (unfold set3_typ_pre_def set2_typ_pre_def comp_def Abs_typ_pre_inverse[OF UNIV_I] map_sum.simps
+  apply (unfold Type.TT_injects0)
+  apply (unfold set3_Type_pre_def set2_Type_pre_def comp_def Abs_Type_pre_inverse[OF UNIV_I] map_sum.simps
     map_prod_simp sum_set_simps prod_set_simps cSup_singleton Un_empty_left Un_empty_right
-    Union_empty image_insert image_empty map_typ_pre_def id_def)
+    Union_empty image_insert image_empty map_Type_pre_def id_def)
   apply (rule exI[of _ \<sigma>])
   apply (rule conjI assms)+
    apply (unfold id_on_def atomize_all atomize_imp)[1]
@@ -89,27 +89,27 @@ lemma Forall_rrename:
   apply (rule refl)
   done
 
-lemma Forall_swap: "y \<notin> FFVars_typ T2 - {x} \<Longrightarrow> Forall (x::'a::var_typ_pre) T1 T2 = Forall y T1 (rrename_typ (id(x:=y,y:=x)) T2)"
+lemma Forall_swap: "y \<notin> FFVars_Type T2 - {x} \<Longrightarrow> Forall (x::'a::var_Type_pre) T1 T2 = Forall y T1 (rrename_Type (id(x:=y,y:=x)) T2)"
   apply (rule trans)
    apply (rule Forall_rrename)
      apply (rule bij_swap[of x y])
     apply (rule supp_swap_bound)
-    apply (rule cinfinite_imp_infinite[OF typ.UNIV_cinfinite])
+    apply (rule cinfinite_imp_infinite[OF Type.UNIV_cinfinite])
   by auto
 
 (* Monomorphising: *)
-instance var :: var_typ_pre apply standard
+instance var :: var_Type_pre apply standard
   using Field_natLeq infinite_iff_card_of_nat infinite_var
   by (auto simp add: regularCard_var)
 
-type_synonym type = "var typ"
+type_synonym type = "var Type"
 type_synonym \<Gamma>\<^sub>\<tau> = "(var \<times> type) list"
 
 definition map_context :: "(var \<Rightarrow> var) \<Rightarrow> \<Gamma>\<^sub>\<tau> \<Rightarrow> \<Gamma>\<^sub>\<tau>" where
-  "map_context f \<equiv> map (map_prod f (rrename_typ f))"
+  "map_context f \<equiv> map (map_prod f (rrename_Type f))"
 
 abbreviation FFVars_ctxt :: "\<Gamma>\<^sub>\<tau> \<Rightarrow> var set" where
-  "FFVars_ctxt xs \<equiv> \<Union>(FFVars_typ ` snd ` set xs)"
+  "FFVars_ctxt xs \<equiv> \<Union>(FFVars_Type ` snd ` set xs)"
 abbreviation extend :: "\<Gamma>\<^sub>\<tau> \<Rightarrow> var \<Rightarrow> type \<Rightarrow> \<Gamma>\<^sub>\<tau>" ("_ ,, _ <: _" [57,75,75] 71) where
   "extend \<Gamma> x T \<equiv> (x, T)#\<Gamma>"
 abbreviation concat :: "\<Gamma>\<^sub>\<tau> \<Rightarrow> \<Gamma>\<^sub>\<tau> \<Rightarrow> \<Gamma>\<^sub>\<tau>" (infixl "(,,)" 71) where
@@ -126,7 +126,7 @@ lemma map_context_comp0[simp]:
   shows "map_context f \<circ> map_context g = map_context (f \<circ> g)"
   apply (rule ext)
   unfolding map_context_def
-  using assms by (auto simp: typ.rrename_comps)
+  using assms by (auto simp: Type.rrename_comps)
 lemmas map_context_comp = trans[OF comp_apply[symmetric] fun_cong[OF map_context_comp0]]
 declare map_context_comp[simp]
 lemma context_dom_set[simp]:
@@ -136,7 +136,7 @@ lemma context_dom_set[simp]:
 lemma set_bd_UNIV: "|set xs| <o |UNIV::var set|"
   apply (rule ordLess_ordLeq_trans)
     apply (tactic \<open>resolve_tac @{context} (BNF_Def.set_bd_of_bnf (the (BNF_Def.bnf_of @{context} @{type_name list}))) 1\<close>)
-  apply (rule var_typ_pre_class.large)
+  apply (rule var_Type_pre_class.large)
   done
 lemma context_set_bd_UNIV[simp]: "|dom xs| <o |UNIV::var set|"
   apply (rule ordLeq_ordLess_trans[OF card_of_image])
@@ -151,7 +151,7 @@ shows "map_context f \<Gamma> = \<Gamma>"
    apply (rule list.map_cong0[of _ _ id])
    apply (rule trans)
     apply (rule prod.map_cong0[of _ _ id _ id])
-  using assms by (fastforce intro!: typ.rrename_cong_ids)+
+  using assms by (fastforce intro!: Type.rrename_cong_ids)+
 
 notation Fun (infixr "\<rightarrow>" 65)
 notation Forall ("\<forall> _ <: _ . _" [62, 62, 62] 70)
@@ -159,7 +159,7 @@ notation Forall ("\<forall> _ <: _ . _" [62, 62, 62] 70)
 abbreviation in_context :: "var \<Rightarrow> type \<Rightarrow> \<Gamma>\<^sub>\<tau> \<Rightarrow> bool" ("_ <: _ \<in> _" [55,55,55] 60) where
   "x <: t \<in> \<Gamma> \<equiv> (x, t) \<in> set \<Gamma>"
 abbreviation well_scoped :: "type \<Rightarrow> \<Gamma>\<^sub>\<tau> \<Rightarrow> bool" ("_ closed'_in _" [55, 55] 60) where
-  "well_scoped S \<Gamma> \<equiv> FFVars_typ S \<subseteq> dom \<Gamma>"
+  "well_scoped S \<Gamma> \<equiv> FFVars_Type S \<subseteq> dom \<Gamma>"
 
 hide_const wf
 inductive wf :: "\<Gamma>\<^sub>\<tau> \<Rightarrow> bool"  where
@@ -173,18 +173,18 @@ print_theorems
 
 lemma in_context_eqvt:
   assumes "bij f" "|supp f| <o |UNIV::var set|"
-  shows "x <: T \<in> \<Gamma> \<Longrightarrow> f x <: rrename_typ f T \<in> map_context f \<Gamma>"
+  shows "x <: T \<in> \<Gamma> \<Longrightarrow> f x <: rrename_Type f T \<in> map_context f \<Gamma>"
   using assms unfolding map_context_def by auto
 
 lemma extend_eqvt:
   assumes "bij f" "|supp f| <o |UNIV::var set|"
-  shows "map_context f (\<Gamma>,,x<:T) = map_context f \<Gamma>,,f x <: rrename_typ f T"
+  shows "map_context f (\<Gamma>,,x<:T) = map_context f \<Gamma>,,f x <: rrename_Type f T"
   using assms unfolding map_context_def by simp
 
 lemma closed_in_eqvt:
   assumes "bij f" "|supp f| <o |UNIV::var set|"
-  shows "S closed_in \<Gamma> \<Longrightarrow> rrename_typ f S closed_in map_context f \<Gamma>"
-  using assms by (auto simp: typ.FFVars_rrenames)
+  shows "S closed_in \<Gamma> \<Longrightarrow> rrename_Type f S closed_in map_context f \<Gamma>"
+  using assms by (auto simp: Type.FFVars_rrenames)
 
 lemma wf_eqvt:
   assumes "bij f" "|supp f| <o |UNIV::var set|"
@@ -197,10 +197,10 @@ unfolding map_context_def proof (induction \<Gamma>)
 qed simp
 
 abbreviation Tsupp :: "\<Gamma>\<^sub>\<tau> \<Rightarrow> type \<Rightarrow> type \<Rightarrow> var set" where
-  "Tsupp \<Gamma> T\<^sub>1 T\<^sub>2 \<equiv> dom \<Gamma> \<union> FFVars_ctxt \<Gamma> \<union> FFVars_typ T\<^sub>1 \<union> FFVars_typ T\<^sub>2"
+  "Tsupp \<Gamma> T\<^sub>1 T\<^sub>2 \<equiv> dom \<Gamma> \<union> FFVars_ctxt \<Gamma> \<union> FFVars_Type T\<^sub>1 \<union> FFVars_Type T\<^sub>2"
 
 lemma small_Tsupp: "small (Tsupp \<Gamma> T\<^sub>1 T\<^sub>2)"
-  by (auto simp: small_def typ.card_of_FFVars_bounds typ.Un_bound var_typ_pre_class.UN_bound set_bd_UNIV typ.set_bd)
+  by (auto simp: small_def Type.card_of_FFVars_bounds Type.Un_bound var_Type_pre_class.UN_bound set_bd_UNIV Type.set_bd)
 
 lemma fresh: "\<exists>xx. xx \<notin> Tsupp \<Gamma> T\<^sub>1 T\<^sub>2"
   by (metis emp_bound equals0D imageI inf.commute inf_absorb2 small_Tsupp small_def small_isPerm subsetI)
@@ -228,13 +228,13 @@ proof-
   thus ?thesis by auto
 qed
 
-lemma rrename_swap_FFvars[simp]: "X \<notin> FFVars_typ T \<Longrightarrow> Y \<notin> FFVars_typ T \<Longrightarrow>
-  rrename_typ (id(X := Y, Y := X)) T = T"
-apply(rule typ.rrename_cong_ids) by auto
+lemma rrename_swap_FFvars[simp]: "X \<notin> FFVars_Type T \<Longrightarrow> Y \<notin> FFVars_Type T \<Longrightarrow>
+  rrename_Type (id(X := Y, Y := X)) T = T"
+apply(rule Type.rrename_cong_ids) by auto
 
 lemma map_context_swap_FFVars[simp]:
-"\<forall>k\<in>set \<Gamma>. X \<noteq> fst k \<and> X \<notin> FFVars_typ (snd k) \<and>
-           Y \<noteq> fst k \<and> Y \<notin> FFVars_typ (snd k) \<Longrightarrow>
+"\<forall>k\<in>set \<Gamma>. X \<noteq> fst k \<and> X \<notin> FFVars_Type (snd k) \<and>
+           Y \<noteq> fst k \<and> Y \<notin> FFVars_Type (snd k) \<Longrightarrow>
     map_context (id(X := Y, Y := X)) \<Gamma> = \<Gamma>"
   unfolding map_context_def apply(rule map_idI) by auto
 
@@ -272,24 +272,24 @@ lemma well_scoped:
 using assms proof (induction \<Gamma> S T rule: ty.induct)
 case (SA_Trans_TVar x U \<Gamma> T) {
   case 1 then show ?case using SA_Trans_TVar
-    by (metis fst_conv imageI singletonD subsetI typ.set(1))
+    by (metis fst_conv imageI singletonD subsetI Type.set(1))
 next
   case 2 then show ?case using SA_Trans_TVar by simp
 } qed auto
 
 declare ty.intros[intro]
 
-lemma ty_fresh_extend: "\<Gamma>,, x <: U \<turnstile> S <: T \<Longrightarrow> x \<notin> dom \<Gamma> \<union> FFVars_ctxt \<Gamma> \<and> x \<notin> FFVars_typ U"
+lemma ty_fresh_extend: "\<Gamma>,, x <: U \<turnstile> S <: T \<Longrightarrow> x \<notin> dom \<Gamma> \<union> FFVars_ctxt \<Gamma> \<and> x \<notin> FFVars_Type U"
   by (metis (no_types, lifting) UnE fst_conv snd_conv subsetD wf_ConsE wf_FFVars wf_context)
 
 make_binder_inductive ty
   subgoal for R B \<sigma> \<Gamma> T1 T2
     unfolding split_beta
     by (elim disj_forward exE)
-      (auto simp add: isPerm_def supp_inv_bound map_context_def[symmetric] typ_vvsubst_rrename
-        typ.rrename_comps typ.FFVars_rrenames wf_eqvt extend_eqvt
+      (auto simp add: isPerm_def supp_inv_bound map_context_def[symmetric] Type_vvsubst_rrename
+        Type.rrename_comps Type.FFVars_rrenames wf_eqvt extend_eqvt
         | ((rule exI[of _ "\<sigma> _"] exI)+, (rule conjI)?, rule refl)
-        | ((rule exI[of _ "rrename_typ \<sigma> _"])+, (rule conjI)?, rule in_context_eqvt))+
+        | ((rule exI[of _ "rrename_Type \<sigma> _"])+, (rule conjI)?, rule in_context_eqvt))+
   subgoal premises prems for R B \<Gamma> T1 T2
     using prems
     unfolding ex_push_inwards conj_disj_distribL ex_disj_distrib
@@ -314,7 +314,7 @@ make_binder_inductive ty
          apply (drule prems(2)[rule_format, of "id(X := Z, Z := X)" "\<Gamma>,, X <: T\<^sub>1" "S\<^sub>2" "T\<^sub>2", rotated 2])
            apply (auto simp: extend_eqvt)
         apply(rule cong[OF cong[OF cong], THEN iffD1, of R , OF refl, rotated -1, 
-          of _ "rrename_typ (id(X := Z, Z := X)) S\<^sub>2"]) 
+          of _ "rrename_Type (id(X := Z, Z := X)) S\<^sub>2"]) 
           apply (drule ty_fresh_extend)
           apply (simp_all add: supp_swap_bound)
           by (metis (no_types, opaque_lifting) image_iff map_context_def map_context_swap_FFVars)
